spki/tcb/coq/spki_tcb_extracted.ml
@@ -1,0 +1,477 @@
+
+(** val negb : bool -> bool **)
+
+let negb = function
+| true -> false
+| false -> true
+
+(** val length : 'a1 list -> int **)
+
+let rec length = function
+| [] -> 0
+| _::l' -> succ (length l')
+
+(** val app : 'a1 list -> 'a1 list -> 'a1 list **)
+
+let rec app l m =
+  match l with
+  | [] -> m
+  | a::l1 -> a::(app l1 m)
+
+type comparison =
+| Eq
+| Lt
+| Gt
+
+module Nat =
+ struct
+  (** val eqb : int -> int -> bool **)
+
+  let rec eqb n m =
+    (fun fO fS n -> if n=0 then fO () else fS (n-1))
+      (fun _ ->
+      (fun fO fS n -> if n=0 then fO () else fS (n-1))
+        (fun _ -> true)
+        (fun _ -> false)
+        m)
+      (fun n' ->
+      (fun fO fS n -> if n=0 then fO () else fS (n-1))
+        (fun _ -> false)
+        (fun m' -> eqb n' m')
+        m)
+      n
+
+  (** val leb : int -> int -> bool **)
+
+  let rec leb n m =
+    (fun fO fS n -> if n=0 then fO () else fS (n-1))
+      (fun _ -> true)
+      (fun n' ->
+      (fun fO fS n -> if n=0 then fO () else fS (n-1))
+        (fun _ -> false)
+        (fun m' -> leb n' m')
+        m)
+      n
+
+  (** val max : int -> int -> int **)
+
+  let rec max n m =
+    (fun fO fS n -> if n=0 then fO () else fS (n-1))
+      (fun _ -> m)
+      (fun n' ->
+      (fun fO fS n -> if n=0 then fO () else fS (n-1))
+        (fun _ -> n)
+        (fun m' -> succ (max n' m'))
+        m)
+      n
+ end
+
+module Pos =
+ struct
+  (** val compare_cont : comparison -> int -> int -> comparison **)
+
+  let rec compare_cont = fun c x y -> if x=y then c else if x<y then Lt else Gt
+
+  (** val compare : int -> int -> comparison **)
+
+  let compare = fun x y -> if x=y then Eq else if x<y then Lt else Gt
+
+  (** val eqb : int -> int -> bool **)
+
+  let rec eqb p q =
+    (fun f2p1 f2p f1 p ->
+  if p<=1 then f1 () else if p mod 2 = 0 then f2p (p/2) else f2p1 (p/2))
+      (fun p0 ->
+      (fun f2p1 f2p f1 p ->
+  if p<=1 then f1 () else if p mod 2 = 0 then f2p (p/2) else f2p1 (p/2))
+        (fun q0 -> eqb p0 q0)
+        (fun _ -> false)
+        (fun _ -> false)
+        q)
+      (fun p0 ->
+      (fun f2p1 f2p f1 p ->
+  if p<=1 then f1 () else if p mod 2 = 0 then f2p (p/2) else f2p1 (p/2))
+        (fun _ -> false)
+        (fun q0 -> eqb p0 q0)
+        (fun _ -> false)
+        q)
+      (fun _ ->
+      (fun f2p1 f2p f1 p ->
+  if p<=1 then f1 () else if p mod 2 = 0 then f2p (p/2) else f2p1 (p/2))
+        (fun _ -> false)
+        (fun _ -> false)
+        (fun _ -> true)
+        q)
+      p
+ end
+
+(** val last : 'a1 list -> 'a1 -> 'a1 **)
+
+let rec last l d =
+  match l with
+  | [] -> d
+  | a::l0 -> (match l0 with
+              | [] -> a
+              | _::_ -> last l0 d)
+
+(** val flat_map : ('a1 -> 'a2 list) -> 'a1 list -> 'a2 list **)
+
+let rec flat_map f = function
+| [] -> []
+| x::t -> app (f x) (flat_map f t)
+
+(** val existsb : ('a1 -> bool) -> 'a1 list -> bool **)
+
+let rec existsb f = function
+| [] -> false
+| a::l0 -> (||) (f a) (existsb f l0)
+
+(** val filter : ('a1 -> bool) -> 'a1 list -> 'a1 list **)
+
+let rec filter f = function
+| [] -> []
+| x::l0 -> if f x then x::(filter f l0) else filter f l0
+
+(** val find : ('a1 -> bool) -> 'a1 list -> 'a1 option **)
+
+let rec find f = function
+| [] -> None
+| x::tl -> if f x then Some x else find f tl
+
+module Z =
+ struct
+  (** val compare : int -> int -> comparison **)
+
+  let compare = fun x y -> if x=y then Eq else if x<y then Lt else Gt
+
+  (** val leb : int -> int -> bool **)
+
+  let leb x y =
+    match compare x y with
+    | Gt -> false
+    | _ -> true
+
+  (** val eqb : int -> int -> bool **)
+
+  let eqb x y =
+    (fun f0 fp fn z -> if z=0 then f0 () else if z>0 then fp z else fn (-z))
+      (fun _ ->
+      (fun f0 fp fn z -> if z=0 then f0 () else if z>0 then fp z else fn (-z))
+        (fun _ -> true)
+        (fun _ -> false)
+        (fun _ -> false)
+        y)
+      (fun p ->
+      (fun f0 fp fn z -> if z=0 then f0 () else if z>0 then fp z else fn (-z))
+        (fun _ -> false)
+        (fun q -> Pos.eqb p q)
+        (fun _ -> false)
+        y)
+      (fun p ->
+      (fun f0 fp fn z -> if z=0 then f0 () else if z>0 then fp z else fn (-z))
+        (fun _ -> false)
+        (fun _ -> false)
+        (fun q -> Pos.eqb p q)
+        y)
+      x
+
+  (** val max : int -> int -> int **)
+
+  let max = Stdlib.max
+
+  (** val min : int -> int -> int **)
+
+  let min = Stdlib.min
+ end
+
+(** val eqb0 : char list -> char list -> bool **)
+
+let rec eqb0 s1 s2 =
+  match s1 with
+  | [] -> (match s2 with
+           | [] -> true
+           | _::_ -> false)
+  | c1::s1' ->
+    (match s2 with
+     | [] -> false
+     | c2::s2' -> if (=) c1 c2 then eqb0 s1' s2' else false)
+
+(** val filter_map : ('a1 -> 'a2 option) -> 'a1 list -> 'a2 list **)
+
+let rec filter_map f = function
+| [] -> []
+| x::xs ->
+  (match f x with
+   | Some y -> y::(filter_map f xs)
+   | None -> filter_map f xs)
+
+type bytes = int list
+
+(** val bytes_eq : bytes -> bytes -> bool **)
+
+let bytes_eq = Spki_tcb.constant_time_compare
+
+(** val sha512 : bytes -> bytes **)
+
+let sha512 = Spki_tcb.sha512_hash
+
+(** val ed25519_verify : bytes -> bytes -> bytes -> bool **)
+
+let ed25519_verify = Spki_tcb.ed25519_verify
+
+type principal =
+| Key of bytes
+| KeyHash of bytes
+
+(** val principal_of_key : bytes -> principal **)
+
+let principal_of_key pk =
+  KeyHash (sha512 pk)
+
+(** val principal_equal : principal -> principal -> bool **)
+
+let principal_equal p1 p2 =
+  match p1 with
+  | Key k ->
+    (match p2 with
+     | Key k2 -> bytes_eq k k2
+     | KeyHash h -> bytes_eq (sha512 k) h)
+  | KeyHash h ->
+    (match p2 with
+     | Key k -> bytes_eq h (sha512 k)
+     | KeyHash h2 -> bytes_eq h h2)
+
+type tag =
+| TagAll
+| TagSet of char list list
+| TagPrefix of char list * tag
+| TagRange of int * int
+| TagThreshold of int * tag list
+
+(** val tag_intersect : tag -> tag -> tag option **)
+
+let rec tag_intersect t1 t2 =
+  match t1 with
+  | TagAll -> Some t2
+  | TagSet s1 ->
+    (match t2 with
+     | TagAll -> Some t1
+     | TagSet s2 ->
+       let common = filter (fun x -> existsb (eqb0 x) s2) s1 in
+       (match common with
+        | [] -> None
+        | _::_ -> Some (TagSet common))
+     | _ -> None)
+  | TagPrefix (n1, sub1) ->
+    (match t2 with
+     | TagAll -> Some t1
+     | TagPrefix (n2, sub2) ->
+       if eqb0 n1 n2
+       then (match tag_intersect sub1 sub2 with
+             | Some sub -> Some (TagPrefix (n1, sub))
+             | None -> None)
+       else None
+     | _ -> None)
+  | TagRange (lo1, hi1) ->
+    (match t2 with
+     | TagAll -> Some t1
+     | TagRange (lo2, hi2) ->
+       let lo = Z.max lo1 lo2 in
+       let hi = Z.min hi1 hi2 in
+       if Z.leb lo hi then Some (TagRange (lo, hi)) else None
+     | _ -> None)
+  | TagThreshold (k1, tags1) ->
+    (match t2 with
+     | TagAll -> Some t1
+     | TagThreshold (k2, tags2) ->
+       let k = Nat.max k1 k2 in
+       let merged =
+         flat_map (fun t3 -> filter_map (tag_intersect t3) tags2) tags1
+       in
+       if Nat.leb k (length merged)
+       then Some (TagThreshold (k, merged))
+       else None
+     | _ -> None)
+
+(** val string_list_eq : char list list -> char list list -> bool **)
+
+let rec string_list_eq l1 l2 =
+  match l1 with
+  | [] -> (match l2 with
+           | [] -> true
+           | _::_ -> false)
+  | s1::rest1 ->
+    (match l2 with
+     | [] -> false
+     | s2::rest2 -> (&&) (eqb0 s1 s2) (string_list_eq rest1 rest2))
+
+(** val tag_list_eq_aux :
+    (tag -> tag -> bool) -> tag list -> tag list -> bool **)
+
+let rec tag_list_eq_aux teq l1 l2 =
+  match l1 with
+  | [] -> (match l2 with
+           | [] -> true
+           | _::_ -> false)
+  | t1::r1 ->
+    (match l2 with
+     | [] -> false
+     | t2::r2 -> (&&) (teq t1 t2) (tag_list_eq_aux teq r1 r2))
+
+(** val tag_eq : tag -> tag -> bool **)
+
+let rec tag_eq t1 t2 =
+  match t1 with
+  | TagAll -> (match t2 with
+               | TagAll -> true
+               | _ -> false)
+  | TagSet s1 ->
+    (match t2 with
+     | TagSet s2 -> string_list_eq s1 s2
+     | _ -> false)
+  | TagPrefix (n1, sub1) ->
+    (match t2 with
+     | TagPrefix (n2, sub2) -> (&&) (eqb0 n1 n2) (tag_eq sub1 sub2)
+     | _ -> false)
+  | TagRange (lo1, hi1) ->
+    (match t2 with
+     | TagRange (lo2, hi2) -> (&&) (Z.eqb lo1 lo2) (Z.eqb hi1 hi2)
+     | _ -> false)
+  | TagThreshold (k1, tags1) ->
+    (match t2 with
+     | TagThreshold (k2, tags2) ->
+       (&&) (Nat.eqb k1 k2) (tag_list_eq_aux tag_eq tags1 tags2)
+     | _ -> false)
+
+(** val tag_subset : tag -> tag -> bool **)
+
+let tag_subset t1 t2 =
+  match tag_intersect t1 t2 with
+  | Some result -> tag_eq result t1
+  | None -> false
+
+type validity =
+| ValidAlways
+| ValidNotBefore of int
+| ValidNotAfter of int
+| ValidBetween of int * int
+
+type cert = { issuer : principal; subject : principal; cert_tag : tag;
+              valid : validity; propagate : bool }
+
+type signed_cert = { the_cert : cert; signature : bytes; cert_hash : bytes }
+
+(** val dummy_cert : cert **)
+
+let dummy_cert =
+  { issuer = (Key []); subject = (Key []); cert_tag = TagAll; valid =
+    ValidAlways; propagate = false }
+
+(** val dummy_signed_cert : signed_cert **)
+
+let dummy_signed_cert =
+  { the_cert = dummy_cert; signature = []; cert_hash = [] }
+
+(** val cert_valid_now : signed_cert -> int -> bool **)
+
+let cert_valid_now sc now =
+  match sc.the_cert.valid with
+  | ValidAlways -> true
+  | ValidNotBefore t -> Z.leb t now
+  | ValidNotAfter t -> Z.leb now t
+  | ValidBetween (t1, t2) -> (&&) (Z.leb t1 now) (Z.leb now t2)
+
+(** val verify_cert_signature : signed_cert -> bytes -> bool **)
+
+let verify_cert_signature sc pk =
+  ed25519_verify pk sc.cert_hash sc.signature
+
+type chain_result =
+| ChainValid of tag
+| ChainInvalid of char list
+
+(** val find_key : principal -> bytes list -> bytes option **)
+
+let find_key p roots =
+  match p with
+  | Key pk -> if existsb (bytes_eq pk) roots then Some pk else None
+  | KeyHash h -> find (fun pk -> bytes_eq (sha512 pk) h) roots
+
+(** val verify_chain_step :
+    signed_cert list -> principal -> tag -> bytes list -> int -> chain_result **)
+
+let rec verify_chain_step certs current_principal current_tag roots now =
+  match certs with
+  | [] -> ChainValid current_tag
+  | sc::rest ->
+    if negb (principal_equal sc.the_cert.issuer current_principal)
+    then ChainInvalid
+           ('i'::('s'::('s'::('u'::('e'::('r'::(' '::('m'::('i'::('s'::('m'::('a'::('t'::('c'::('h'::[])))))))))))))))
+    else (match find_key sc.the_cert.issuer roots with
+          | Some pk ->
+            if negb (verify_cert_signature sc pk)
+            then ChainInvalid
+                   ('s'::('i'::('g'::('n'::('a'::('t'::('u'::('r'::('e'::(' '::('i'::('n'::('v'::('a'::('l'::('i'::('d'::[])))))))))))))))))
+            else if negb (cert_valid_now sc now)
+                 then ChainInvalid
+                        ('c'::('e'::('r'::('t'::(' '::('e'::('x'::('p'::('i'::('r'::('e'::('d'::[]))))))))))))
+                 else if (&&) (negb sc.the_cert.propagate)
+                           (negb (match rest with
+                                  | [] -> true
+                                  | _::_ -> false))
+                      then ChainInvalid
+                             ('d'::('e'::('l'::('e'::('g'::('a'::('t'::('i'::('o'::('n'::(' '::('n'::('o'::('t'::(' '::('p'::('e'::('r'::('m'::('i'::('t'::('t'::('e'::('d'::[]))))))))))))))))))))))))
+                      else (match tag_intersect current_tag
+                                    sc.the_cert.cert_tag with
+                            | Some new_tag ->
+                              verify_chain_step rest sc.the_cert.subject
+                                new_tag roots now
+                            | None ->
+                              ChainInvalid
+                                ('n'::('o'::(' '::('c'::('o'::('m'::('m'::('o'::('n'::(' '::('c'::('a'::('p'::('a'::('b'::('i'::('l'::('i'::('t'::('i'::('e'::('s'::[])))))))))))))))))))))))
+          | None ->
+            ChainInvalid
+              ('u'::('n'::('k'::('n'::('o'::('w'::('n'::(' '::('i'::('s'::('s'::('u'::('e'::('r'::[])))))))))))))))
+
+(** val verify_chain :
+    signed_cert list -> bytes list -> int -> chain_result **)
+
+let verify_chain chain0 roots now =
+  match chain0 with
+  | [] ->
+    ChainInvalid
+      ('e'::('m'::('p'::('t'::('y'::(' '::('c'::('h'::('a'::('i'::('n'::[])))))))))))
+  | first::_ ->
+    let root_principal = first.the_cert.issuer in
+    (match find_key root_principal roots with
+     | Some _ -> verify_chain_step chain0 root_principal TagAll roots now
+     | None ->
+       ChainInvalid
+         ('r'::('o'::('o'::('t'::(' '::('n'::('o'::('t'::(' '::('t'::('r'::('u'::('s'::('t'::('e'::('d'::[])))))))))))))))))
+
+type auth_request = { requester : principal; action : char list;
+                      resource : char list; chain : signed_cert list }
+
+type auth_result =
+| Authorized of tag
+| Denied of char list
+
+(** val authorize : auth_request -> bytes list -> int -> auth_result **)
+
+let authorize req roots now =
+  match verify_chain req.chain roots now with
+  | ChainValid t ->
+    (match req.chain with
+     | [] -> Denied ('n'::('o'::(' '::('c'::('h'::('a'::('i'::('n'::[]))))))))
+     | _::_ ->
+       let leaf = last req.chain dummy_signed_cert in
+       if negb (principal_equal leaf.the_cert.subject req.requester)
+       then Denied
+              ('r'::('e'::('q'::('u'::('e'::('s'::('t'::('e'::('r'::(' '::('n'::('o'::('t'::(' '::('a'::('u'::('t'::('h'::('o'::('r'::('i'::('z'::('e'::('d'::[]))))))))))))))))))))))))
+       else let action_tag = TagSet (req.action::[]) in
+            (match tag_intersect t action_tag with
+             | Some _ -> Authorized t
+             | None ->
+               Denied
+                 ('a'::('c'::('t'::('i'::('o'::('n'::(' '::('n'::('o'::('t'::(' '::('p'::('e'::('r'::('m'::('i'::('t'::('t'::('e'::('d'::[]))))))))))))))))))))))
+  | ChainInvalid reason -> Denied reason
