spki/tcb/coq/spki_tcb_extracted.mli
@@ -1,0 +1,128 @@
+
+val negb : bool -> bool
+
+val length : 'a1 list -> int
+
+val app : 'a1 list -> 'a1 list -> 'a1 list
+
+type comparison =
+| Eq
+| Lt
+| Gt
+
+module Nat :
+ sig
+  val eqb : int -> int -> bool
+
+  val leb : int -> int -> bool
+
+  val max : int -> int -> int
+ end
+
+module Pos :
+ sig
+  val compare_cont : comparison -> int -> int -> comparison
+
+  val compare : int -> int -> comparison
+
+  val eqb : int -> int -> bool
+ end
+
+val last : 'a1 list -> 'a1 -> 'a1
+
+val flat_map : ('a1 -> 'a2 list) -> 'a1 list -> 'a2 list
+
+val existsb : ('a1 -> bool) -> 'a1 list -> bool
+
+val filter : ('a1 -> bool) -> 'a1 list -> 'a1 list
+
+val find : ('a1 -> bool) -> 'a1 list -> 'a1 option
+
+module Z :
+ sig
+  val compare : int -> int -> comparison
+
+  val leb : int -> int -> bool
+
+  val eqb : int -> int -> bool
+
+  val max : int -> int -> int
+
+  val min : int -> int -> int
+ end
+
+val eqb0 : char list -> char list -> bool
+
+val filter_map : ('a1 -> 'a2 option) -> 'a1 list -> 'a2 list
+
+type bytes = int list
+
+val bytes_eq : bytes -> bytes -> bool
+
+val sha512 : bytes -> bytes
+
+val ed25519_verify : bytes -> bytes -> bytes -> bool
+
+type principal =
+| Key of bytes
+| KeyHash of bytes
+
+val principal_of_key : bytes -> principal
+
+val principal_equal : principal -> principal -> bool
+
+type tag =
+| TagAll
+| TagSet of char list list
+| TagPrefix of char list * tag
+| TagRange of int * int
+| TagThreshold of int * tag list
+
+val tag_intersect : tag -> tag -> tag option
+
+val string_list_eq : char list list -> char list list -> bool
+
+val tag_list_eq_aux : (tag -> tag -> bool) -> tag list -> tag list -> bool
+
+val tag_eq : tag -> tag -> bool
+
+val tag_subset : tag -> tag -> bool
+
+type validity =
+| ValidAlways
+| ValidNotBefore of int
+| ValidNotAfter of int
+| ValidBetween of int * int
+
+type cert = { issuer : principal; subject : principal; cert_tag : tag;
+              valid : validity; propagate : bool }
+
+type signed_cert = { the_cert : cert; signature : bytes; cert_hash : bytes }
+
+val dummy_cert : cert
+
+val dummy_signed_cert : signed_cert
+
+val cert_valid_now : signed_cert -> int -> bool
+
+val verify_cert_signature : signed_cert -> bytes -> bool
+
+type chain_result =
+| ChainValid of tag
+| ChainInvalid of char list
+
+val find_key : principal -> bytes list -> bytes option
+
+val verify_chain_step :
+  signed_cert list -> principal -> tag -> bytes list -> int -> chain_result
+
+val verify_chain : signed_cert list -> bytes list -> int -> chain_result
+
+type auth_request = { requester : principal; action : char list;
+                      resource : char list; chain : signed_cert list }
+
+type auth_result =
+| Authorized of tag
+| Denied of char list
+
+val authorize : auth_request -> bytes list -> int -> auth_result
